solved

HumanEvalLean/HumanEval130.lean
@@ -1,5 +1,245 @@
-def tri : Unit :=
-  ()
+import Std
+import Lean.LibrarySuggestions.Default
+open Std Std.Do
+
+set_option mvcgen.warning false
+
+/-!
+## Implementation
+-/
+
+-- def tri (n : Nat) : List Nat := Id.run do
+--   let mut xs : Array Nat := #[]
+--   let mut lastₑ := 1
+--   let mut lastₒ := 0
+--   for i in 0...=n do
+--     (xs, lastₑ, lastₒ) := (go i xs lastₑ lastₒ).run
+--   return xs.toList
+-- where
+--   @[inline]
+--   go (i : Nat) (xs : Array Nat) (lastₑ lastₒ : Nat) : Id (Array Nat × Nat × Nat) := do
+--     if i % 2 == 0 then
+--       let lastₑ := i / 2 + 1
+--       return (xs.push lastₑ, lastₑ, lastₒ)
+--     else
+--       let lastₒ := lastₑ + lastₒ + (i + 3) / 2
+--       return (xs.push lastₒ, lastₑ, lastₒ)
+
+def tri (n : Nat) : List Nat := Id.run do
+  let mut xs : Array Nat := #[]
+  let mut lastₑ := 1
+  let mut lastₒ := 0
+  for i in 0...=n do
+    if i % 2 == 0 then
+      lastₑ := i / 2 + 1
+      xs := xs.push lastₑ
+    else
+      lastₒ := (lastₑ + lastₒ + (i + 3) / 2)
+      xs := xs.push lastₒ
+  return xs.toList
+
+-- def tri (n : Nat) : List Nat :=
+--   (go 0 1 0 #[]).toList
+-- where
+--   go (i : Nat) (lastₑ lastₒ : Nat) (acc : Array Nat) : Array Nat :=
+--     if i ≤ n then
+--       if i % 2 == 0 then
+--         let lastₑ := i / 2 + 1
+--         go (i + 1) lastₑ lastₒ (acc.push lastₑ)
+--       else
+--         let lastₒ := lastₑ + lastₒ + (i + 3) / 2
+--         go (i + 1) lastₑ lastₒ (acc.push lastₒ)
+--     else
+--       acc
+--   termination_by n + 1 - i
+
+/-!
+## Tests
+-/
+
+example : tri 3 = [1, 3, 2, 8] := by native_decide
+example : tri 4 = [1, 3, 2, 8, 3] := by native_decide
+example : tri 5 = [1, 3, 2, 8, 3, 15] := by native_decide
+example : tri 6 = [1, 3, 2, 8, 3, 15, 4] := by native_decide
+example : tri 7 = [1, 3, 2, 8, 3, 15, 4, 24] := by native_decide
+example : tri 8 = [1, 3, 2, 8, 3, 15, 4, 24, 5] := by native_decide
+example : tri 9 = [1, 3, 2, 8, 3, 15, 4, 24, 5, 35] := by native_decide
+example : tri 20 = [1, 3, 2, 8, 3, 15, 4, 24, 5, 35, 6, 48, 7, 63, 8, 80, 9, 99, 10, 120, 11] := by native_decide
+example : tri 0 = [1] := by native_decide
+example : tri 1 = [1, 3] := by native_decide
+
+/-!
+## Verification
+-/
+
+-- theorem length_triGo :
+--     (tri.go n i lastₑ lastₒ acc).size = acc.size + (n + 1 - i) := by
+--   sorry
+
+/-
+      ⌜(cur.pos < 2 → (lastₑ, lastₒ) = (1, 0)) ∧
+        ∃ (h : xs.size = cur.pos), (_ : 2 ≤ cur.pos) →
+          (∀ i, (h : i = cur.pos - 1 ∨ i = cur.pos - 2) → if i % 2 = 0 then lastₑ = xs[i] else lastₒ = xs[i]) ∧
+          ((_ : 0 < cur.pos) → xs[0] = 1) ∧ ((_ : 1 < cur.pos) → xs[1] = 3) ∧
+          (∀ i, (_ : i + 2 < cur.pos) → if i % 2 = 0 then xs[i + 2] = 1 + n / 2 else xs[i + 2] = xs[i] + xs[i + 1] + (i + 5) / 2)⌝
+-/
+
+def Inv₁ (cur : (0...=n).toList.Cursor) (lastₑ lastₒ : Nat) (xs : Array Nat) : Prop :=
+  xs.size = cur.pos
+
+def Inv₂ (cur : (0...=n).toList.Cursor) (lastₑ lastₒ : Nat) (xs : Array Nat) : Prop :=
+  xs.size < 2 → (lastₑ, lastₒ) = (1, 0)
+
+def Inv₃ (cur : (0...=n).toList.Cursor) (lastₑ lastₒ : Nat) (xs : Array Nat) : Prop :=
+  ∀ (_ : 2 ≤ xs.size) (i : Nat) (_ : i = xs.size - 2 ∨ i = xs.size - 1),
+    if i % 2 = 0 then lastₑ = xs[i] else lastₒ = xs[i]
+
+def Inv₄ (cur : (0...=n).toList.Cursor) (lastₑ lastₒ : Nat) (xs : Array Nat) : Prop :=
+  ((_ : 0 < xs.size) → xs[0] = 1) ∧ ((_ : 1 < xs.size) → xs[1] = 3)
+
+def Inv₅ (cur : (0...=n).toList.Cursor) (lastₑ lastₒ : Nat) (xs : Array Nat) : Prop :=
+  ∀ (i : Nat) (_ : i + 2 < xs.size),
+    if i % 2 = 0 then xs[i + 2] = 1 + (i + 2) / 2 else xs[i + 2] = xs[i] + xs[i + 1] + (i + 5) / 2
+
+-- theorem inv₁ (h₁ : inv₁ )
+
+theorem Nat.eq_add_of_toList_rcc_eq_append_cons {a b : Nat} {pref cur suff}
+    (h : (a...=b).toList = pref ++ cur :: suff) :
+    cur = a + pref.length := by
+  have := Rcc.eq_succMany?_of_toList_eq_append_cons h
+  grind [PRange.Nat.succMany?_eq]
+
+@[simp, grind =]
+theorem length_tri : (tri n).length = n + 1 := by
+  generalize hwp : tri n = wp
+  apply Id.of_wp_run_eq hwp
+  mvcgen
+  invariants
+  · ⇓⟨cur, lastₑ, lastₒ, xs⟩ => ⌜xs.size = cur.pos⌝
+  with grind [Nat.length_toList_rcc]
+
+theorem bla {n i} {h : i ≤ n} :
+    (tri n)[i]! =
+      if i = 0 then
+        1
+      else if i = 1 then
+        3
+      else if i % 2 = 0 then
+        1 + i / 2
+      else
+        (tri n)[i - 2]! + (tri n)[i - 1]! + (i + 3) / 2 := by
+  let wp := tri n
+  have hwp : tri n = wp := rfl
+  simp only [hwp]
+  clear_value wp
+  apply Id.of_wp_run_eq hwp
+  mvcgen
+  invariants
+  · ⇓⟨cur, lastₑ, lastₒ, xs⟩ =>
+      ⌜Inv₁ cur lastₑ lastₒ xs ∧
+        Inv₂ cur lastₑ lastₒ xs ∧
+        Inv₃ cur lastₑ lastₒ xs ∧
+        Inv₄ cur lastₑ lastₒ xs ∧
+        Inv₅ cur lastₑ lastₒ xs⌝
+  case vc1 pref cur suff h_append_cons args lastₑ args₂ lastₒ' xs hmod lastₑ' xs' hinv =>
+    obtain ⟨h₁, h₂, h₃, h₄, h₅⟩ := hinv
+    have hcur := Nat.eq_add_of_toList_rcc_eq_append_cons h_append_cons
+    refine ⟨?_, ?_, ?_, ?_, ?_⟩
+    · grind [Inv₁]
+    · grind [Inv₁, Inv₂]
+    · simp only [Inv₃] at h₃ ⊢
+      intro hge i hi
+      by_cases xs.size < 2
+      · grind [Inv₁]
+      · by_cases i = xs.size
+        · grind [Inv₁]
+        · specialize h₃ (by grind) i (by grind)
+          grind [Inv₁]
+    · grind [Inv₁, Inv₄]
+    · grind [Inv₁, Inv₅]
+  case vc2 pref cur suff h_append_cons args lastₑ args₂ lastₒ xs hmod lastₒ' xs' hinv =>
+    obtain ⟨h₁, h₂, h₃, h₄, h₅⟩ := hinv
+    have hcur := Nat.eq_add_of_toList_rcc_eq_append_cons h_append_cons
+    refine ⟨?_, ?_, ?_, ?_, ?_⟩
+    · grind [Inv₁]
+    · grind [Inv₁, Inv₂]
+    · simp only [Inv₃] at h₃ ⊢
+      intro hge i hi
+      by_cases xs.size < 2
+      · grind [Inv₂, Inv₄]
+      · by_cases i = xs.size
+        · grind [Inv₁]
+        · specialize h₃ (by grind) i (by grind)
+          grind [Inv₁]
+    · grind [Inv₁, Inv₂, Inv₄]
+    · simp only [Inv₅] at h₅ ⊢
+      intro i hi
+      by_cases i + 2 = xs.size
+      · have : xs'[i + 2] = lastₒ' := by grind
+        simp only [this, lastₒ']
+        have : i % 2 = 1 := by grind [Inv₁]
+        rw [if_neg (by grind [Inv₁])]
+        have : cur = i + 2 := by grind [Inv₁]
+        simp only [Inv₃] at h₃
+        have h₃₁ := h₃ (by grind) (i + 1) (by grind)
+        have h₃₂ := h₃ (by grind) i (by grind)
+        grind
+      · grind
+  case vc3 => grind [Inv₁, Inv₂, Inv₃, Inv₄, Inv₅]
+  case vc4 args hinv =>
+    obtain ⟨h₁, h₂, h₃, h₄, h₅⟩ := hinv
+    have : args.2.2.size = n + 1 := by grind [Inv₁, Nat.length_toList_rcc]
+    split
+    · grind [Inv₄]
+    · split
+      · grind [Inv₄]
+      · simp only [Inv₅] at h₅
+        specialize h₅ (i - 2) (by grind)
+        grind
+
+theorem tri_zero :
+    (tri n)[0] = 1 := by
+  have := bla (n := n) (i := 0) (h := by grind)
+  grind
+
+theorem tri_one (h : 1 ≤ n) :
+    (tri n)[1]'(by grind) = 3 := by
+  have := bla (n := n) (i := 1) (h := h)
+  grind
+
+theorem tri_of_even (h : i ≤ n) (hi : i % 2 = 0) :
+    (tri n)[i]'(by grind) = 1 + (i / 2) := by
+  have := bla (n := n) (i := i) (h := h)
+  grind
+
+/--
+Expresses the value at an even position in terms of its two predecessors.
+-/
+theorem tri_of_odd₁ (h : i ≤ n) (hge : 2 ≤ i) (hi : i % 2 = 1) :
+    (tri n)[i]'(by grind) = (tri n)[i - 2]'(by grind) + (tri n)[i - 1]'(by grind) + (i + 3) / 2 := by
+  have := bla (n := n) (i := i) (h := h)
+  grind
+
+/--
+This is the property specified for the value at even positions:
+It is equal to the sum of its two predecessors and its successor.
+-/
+theorem tri_of_odd₂ (h : i + 1 ≤ n) (hge : 2 ≤ i) (hi : i % 2 = 1) :
+    (tri n)[i]'(by grind) = (tri n)[i - 2]'(by grind) + (tri n)[i - 1]'(by grind) + (tri n)[i + 1]'(by grind) := by
+  grind [tri_of_odd₁, tri_of_even]
+
+theorem prefix_tri_of_le (h : m ≤ n) :
+    tri m <+: tri n := by
+  simp only [List.IsPrefix]
+  refine ⟨(tri n).drop (m + 1), ?_⟩
+  apply List.ext_getElem
+  · grind
+  · intro i _ _
+    by_cases i ≤ m
+    · rw [List.getElem_append_left (by grind)]
+      induction i using Nat.strongRecOn with | ind i ih
+      grind [tri_of_even, tri_of_odd₁, tri_one]
+    · grind
 
 /-!
 ## Prompt
@@ -7,7 +247,7 @@ def tri : Unit :=
 ```python3
 
 def tri(n):
-    """Everyone knows Fibonacci sequence, it was studied deeply by mathematicians in 
+    """Everyone knows Fibonacci sequence, it was studied deeply by mathematicians in
     the last couple centuries. However, what people don't know is Tribonacci sequence.
     Tribonacci sequence is defined by the recurrence:
     tri(1) = 3
@@ -17,8 +257,8 @@ def tri(n):
     tri(2) = 1 + (2 / 2) = 2
     tri(4) = 3
     tri(3) = tri(2) + tri(1) + tri(4)
-           = 2 + 3 + 3 = 8 
-    You are given a non-negative integer number n, you have to a return a list of the 
+           = 2 + 3 + 3 = 8
+    You are given a non-negative integer number n, you have to a return a list of the
     first n + 1 numbers of the Tribonacci sequence.
     Examples:
     tri(3) = [1, 3, 2, 8]
@@ -45,7 +285,7 @@ def tri(n):
 def check(candidate):
 
     # Check some simple cases
-    
+
     assert candidate(3) == [1, 3, 2.0, 8.0]
     assert candidate(4) == [1, 3, 2.0, 8.0, 3.0]
     assert candidate(5) == [1, 3, 2.0, 8.0, 3.0, 15.0]
